Changed NUMERAL_BIT1 and NUMERAL_BIT2 to BIT1 and BIT2, respectively. Sorry, they were just too long. Also, ALT_ZERO is now named ZERO.

src/num/theories/Num_conv.sml
@@ -28,7 +28,7 @@ val numeral_pre     = numeralTheory.numeral_pre
 val numeral_lt      = numeralTheory.numeral_lt
 val numeral_distrib = numeralTheory.numeral_distrib
 val save_zero =
-  prove(Term`NUMERAL ALT_ZERO = 0`,
+  prove(Term`NUMERAL ZERO = 0`,
    REWRITE_TAC [arithmeticTheory.NUMERAL_DEF, arithmeticTheory.ALT_ZERO]);
 
 
