src/num/theories/numeralScript.sml
@@ -57,10 +57,10 @@ val PRE_ADD = prove(
 
 val numeral_suc = store_thm(
   "numeral_suc",
-  Term `(SUC ALT_ZERO = NUMERAL_BIT1 ALT_ZERO) /\
-        (!n. SUC (NUMERAL_BIT1 n) = NUMERAL_BIT2 n) /\
-        (!n. SUC (NUMERAL_BIT2 n) = NUMERAL_BIT1 (SUC n))`,
-  SIMP_TAC bool_ss [NUMERAL_BIT1, NUMERAL_BIT2, ALT_ZERO, ADD_CLAUSES]);
+  Term `(SUC ZERO = BIT1 ZERO) /\
+        (!n. SUC (BIT1 n) = BIT2 n) /\
+        (!n. SUC (BIT2 n) = BIT1 (SUC n))`,
+  SIMP_TAC bool_ss [BIT1, BIT2, ALT_ZERO, ADD_CLAUSES]);
 
 (* internal markers *)
 
@@ -79,22 +79,22 @@ val numeral_distrib = store_thm(
    (!n m. NUMERAL n * NUMERAL m = NUMERAL (n * m)) /\
    (!n. 0 - n = 0) /\ (!n. n - 0 = n) /\
    (!n m. NUMERAL n - NUMERAL m = NUMERAL (n - m)) /\
-   (!n. 0 EXP (NUMERAL (NUMERAL_BIT1 n)) = 0) /\
-   (!n. 0 EXP (NUMERAL (NUMERAL_BIT2 n)) = 0) /\
+   (!n. 0 EXP (NUMERAL (BIT1 n)) = 0) /\
+   (!n. 0 EXP (NUMERAL (BIT2 n)) = 0) /\
    (!n. n EXP 0 = 1) /\
    (!n m. (NUMERAL n) EXP (NUMERAL m) = NUMERAL (n EXP m)) /\
    (SUC 0 = 1) /\
    (!n. SUC(NUMERAL n) = NUMERAL (SUC n)) /\
    (PRE 0 = 0) /\
    (!n. PRE(NUMERAL n) = NUMERAL (PRE n)) /\
-   (!n. (NUMERAL n = 0) = (n = ALT_ZERO)) /\
-   (!n. (0 = NUMERAL n) = (n = ALT_ZERO)) /\
+   (!n. (NUMERAL n = 0) = (n = ZERO)) /\
+   (!n. (0 = NUMERAL n) = (n = ZERO)) /\
    (!n m. (NUMERAL n = NUMERAL m) = (n=m)) /\
-   (!n. n < 0 = F) /\ (!n. 0 < NUMERAL n = ALT_ZERO < n) /\
+   (!n. n < 0 = F) /\ (!n. 0 < NUMERAL n = ZERO < n) /\
    (!n m. NUMERAL n < NUMERAL m  = n<m)  /\
-   (!n. 0 > n = F) /\ (!n. NUMERAL n > 0 = ALT_ZERO < n) /\
+   (!n. 0 > n = F) /\ (!n. NUMERAL n > 0 = ZERO < n) /\
    (!n m. NUMERAL n > NUMERAL m  = m<n)  /\
-   (!n. 0 <= n = T) /\ (!n. NUMERAL n <= 0 = n <= ALT_ZERO) /\
+   (!n. 0 <= n = T) /\ (!n. NUMERAL n <= 0 = n <= ZERO) /\
    (!n m. NUMERAL n <= NUMERAL m = n<=m) /\
    (!n. n >= 0 = T) /\ (!n. 0 >= n = (n = 0)) /\
    (!n m. NUMERAL n >= NUMERAL m = m <= n) /\
@@ -103,16 +103,15 @@ val numeral_distrib = store_thm(
   SIMP_TAC bool_ss [NUMERAL_DEF, GREATER_DEF, iZ, GREATER_OR_EQ,
                     LESS_OR_EQ, EQ_IMP_THM, DISJ_IMP_THM, ADD_CLAUSES,
                     ALT_ZERO, MULT_CLAUSES, EXP, PRE, NOT_LESS_0, SUB_0,
-                    NUMERAL_BIT1, NUMERAL_BIT2, ODD, EVEN] THEN
+                    BIT1, BIT2, ODD, EVEN] THEN
   mesonLib.MESON_TAC [LESS_0_CASES]);
 
 val numeral_iisuc = store_thm(
   "numeral_iisuc", Term
-  `(iiSUC ALT_ZERO = NUMERAL_BIT2 ALT_ZERO) /\
-   (iiSUC (NUMERAL_BIT1 n) = NUMERAL_BIT1 (SUC n)) /\
-   (iiSUC (NUMERAL_BIT2 n) = NUMERAL_BIT2 (SUC n))`,
-  SIMP_TAC bool_ss [NUMERAL_BIT1, NUMERAL_BIT2, iiSUC, ALT_ZERO,
-                    ADD_CLAUSES]);
+  `(iiSUC ZERO = BIT2 ZERO) /\
+   (iiSUC (BIT1 n) = BIT1 (SUC n)) /\
+   (iiSUC (BIT2 n) = BIT2 (SUC n))`,
+  SIMP_TAC bool_ss [BIT1, BIT2, iiSUC, ALT_ZERO, ADD_CLAUSES]);
 
 (* the following addition algorithm makes use of internal markers iZ and
    iiSUC.
@@ -130,35 +129,32 @@ val numeral_add = store_thm(
   "numeral_add",
   Term
   `!n m.
-   (iZ (ALT_ZERO + n) = n) /\ 
-   (iZ (n + ALT_ZERO) = n) /\
-   (iZ (NUMERAL_BIT1 n + NUMERAL_BIT1 m) = NUMERAL_BIT2 (iZ (n + m))) /\
-   (iZ (NUMERAL_BIT1 n + NUMERAL_BIT2 m) = NUMERAL_BIT1 (SUC (n + m))) /\
-   (iZ (NUMERAL_BIT2 n + NUMERAL_BIT1 m) = NUMERAL_BIT1 (SUC (n + m))) /\
-   (iZ (NUMERAL_BIT2 n + NUMERAL_BIT2 m) = NUMERAL_BIT2 (SUC (n + m))) /\
-   (SUC (ALT_ZERO + n) = SUC n) /\ (SUC (n + ALT_ZERO) = SUC n) /\
-   (SUC (NUMERAL_BIT1 n + NUMERAL_BIT1 m) = NUMERAL_BIT1 (SUC (n + m))) /\
-   (SUC (NUMERAL_BIT1 n + NUMERAL_BIT2 m) = NUMERAL_BIT2 (SUC (n + m))) /\
-   (SUC (NUMERAL_BIT2 n + NUMERAL_BIT1 m) = NUMERAL_BIT2 (SUC (n + m))) /\
-   (SUC (NUMERAL_BIT2 n + NUMERAL_BIT2 m) = NUMERAL_BIT1 (iiSUC (n + m))) /\
-   (iiSUC (ALT_ZERO + n) = iiSUC n) /\ (iiSUC (n + ALT_ZERO) = iiSUC n) /\
-   (iiSUC (NUMERAL_BIT1 n + NUMERAL_BIT1 m) =
-      NUMERAL_BIT2 (SUC (n + m))) /\
-   (iiSUC (NUMERAL_BIT1 n + NUMERAL_BIT2 m) =
-      NUMERAL_BIT1 (iiSUC (n + m))) /\
-   (iiSUC (NUMERAL_BIT2 n + NUMERAL_BIT1 m) =
-      NUMERAL_BIT1 (iiSUC (n + m))) /\
-   (iiSUC (NUMERAL_BIT2 n + NUMERAL_BIT2 m) =
-      NUMERAL_BIT2 (iiSUC (n + m)))`,
-  SIMP_TAC bool_ss [NUMERAL_BIT1, NUMERAL_BIT2, iZ, iiSUC,
-                    ADD_CLAUSES, INV_SUC_EQ, ALT_ZERO] THEN
+   (iZ (ZERO + n) = n) /\ 
+   (iZ (n + ZERO) = n) /\
+   (iZ (BIT1 n + BIT1 m) = BIT2 (iZ (n + m))) /\
+   (iZ (BIT1 n + BIT2 m) = BIT1 (SUC (n + m))) /\
+   (iZ (BIT2 n + BIT1 m) = BIT1 (SUC (n + m))) /\
+   (iZ (BIT2 n + BIT2 m) = BIT2 (SUC (n + m))) /\
+   (SUC (ZERO + n) = SUC n) /\ 
+   (SUC (n + ZERO) = SUC n) /\
+   (SUC (BIT1 n + BIT1 m) = BIT1 (SUC (n + m))) /\
+   (SUC (BIT1 n + BIT2 m) = BIT2 (SUC (n + m))) /\
+   (SUC (BIT2 n + BIT1 m) = BIT2 (SUC (n + m))) /\
+   (SUC (BIT2 n + BIT2 m) = BIT1 (iiSUC (n + m))) /\
+   (iiSUC (ZERO + n) = iiSUC n) /\ 
+   (iiSUC (n + ZERO) = iiSUC n) /\
+   (iiSUC (BIT1 n + BIT1 m) = BIT2 (SUC (n + m))) /\
+   (iiSUC (BIT1 n + BIT2 m) = BIT1 (iiSUC (n + m))) /\
+   (iiSUC (BIT2 n + BIT1 m) = BIT1 (iiSUC (n + m))) /\
+   (iiSUC (BIT2 n + BIT2 m) = BIT2 (iiSUC (n + m)))`,
+  SIMP_TAC bool_ss [BIT1, BIT2, iZ, iiSUC,ADD_CLAUSES, INV_SUC_EQ, ALT_ZERO] THEN
   REPEAT GEN_TAC THEN CONV_TAC (AC_CONV(ADD_ASSOC, ADD_SYM)));
 
 (* rewrites needed for addition *)
 
 val add_rwts = [numeral_distrib, numeral_add, numeral_suc, numeral_iisuc]
 
-val numeral_proof_rwts = [NUMERAL_BIT1, NUMERAL_BIT2, INV_SUC_EQ,
+val numeral_proof_rwts = [BIT1, BIT2, INV_SUC_EQ,
                           NUMERAL_DEF, iZ, iiSUC, ADD_CLAUSES, NOT_SUC,
                           SUC_NOT, LESS_0, NOT_LESS_0, ALT_ZERO]
 
@@ -173,12 +169,14 @@ val _ = print "Developing numeral rewrites for relations\n"
 val numeral_eq = store_thm(
   "numeral_eq",
   Term`!n m.
-    ((ALT_ZERO = NUMERAL_BIT1 n) = F) /\ ((NUMERAL_BIT1 n = ALT_ZERO) = F) /\
-    ((ALT_ZERO = NUMERAL_BIT2 n) = F) /\ ((NUMERAL_BIT2 n = ALT_ZERO) = F) /\
-    ((NUMERAL_BIT1 n = NUMERAL_BIT2 m) = F) /\
-    ((NUMERAL_BIT2 n = NUMERAL_BIT1 m) = F) /\
-    ((NUMERAL_BIT1 n = NUMERAL_BIT1 m) = (n = m)) /\
-    ((NUMERAL_BIT2 n = NUMERAL_BIT2 m) = (n = m))`,
+    ((ZERO = BIT1 n) = F) /\ 
+    ((BIT1 n = ZERO) = F) /\
+    ((ZERO = BIT2 n) = F) /\ 
+    ((BIT2 n = ZERO) = F) /\
+    ((BIT1 n = BIT2 m) = F) /\
+    ((BIT2 n = BIT1 m) = F) /\
+    ((BIT1 n = BIT1 m) = (n = m)) /\
+    ((BIT2 n = BIT2 m) = (n = m))`,
   SIMP_TAC bool_ss numeral_proof_rwts THEN
   INDUCT_TAC THEN
   SIMP_TAC bool_ss (double_add_not_SUC::numeral_proof_rwts) THEN
@@ -223,13 +221,13 @@ val numeral_lt = store_thm(
   "numeral_lt",
   Term
   `!n m.
-    (ALT_ZERO < NUMERAL_BIT1 n = T) /\ 
-    (ALT_ZERO < NUMERAL_BIT2 n = T) /\
-    (n < ALT_ZERO = F) /\
-    (NUMERAL_BIT1 n < NUMERAL_BIT1 m = n < m) /\
-    (NUMERAL_BIT2 n < NUMERAL_BIT2 m = n < m) /\
-    (NUMERAL_BIT1 n < NUMERAL_BIT2 m = ~(m < n)) /\
-    (NUMERAL_BIT2 n < NUMERAL_BIT1 m = n < m)`,
+    (ZERO < BIT1 n = T) /\ 
+    (ZERO < BIT2 n = T) /\
+    (n < ZERO = F) /\
+    (BIT1 n < BIT1 m = n < m) /\
+    (BIT2 n < BIT2 m = n < m) /\
+    (BIT1 n < BIT2 m = ~(m < n)) /\
+    (BIT2 n < BIT1 m = n < m)`,
   SIMP_TAC bool_ss (DOUBLE_FACTS::LESS_MONO_EQ::numeral_proof_rwts));
 
 (* I've kept this rewrite entirely independent of the above.  I don't if
@@ -237,13 +235,13 @@ val numeral_lt = store_thm(
 
 val numeral_lte = store_thm(
   "numeral_lte", Term
-  `!n m. (ALT_ZERO <= n = T) /\
-         (NUMERAL_BIT1 n <= ALT_ZERO = F) /\ 
-         (NUMERAL_BIT2 n <= ALT_ZERO = F) /\
-         (NUMERAL_BIT1 n <= NUMERAL_BIT1 m = n <= m) /\
-         (NUMERAL_BIT1 n <= NUMERAL_BIT2 m = n <= m) /\
-         (NUMERAL_BIT2 n <= NUMERAL_BIT1 m = ~(m <= n)) /\
-         (NUMERAL_BIT2 n <= NUMERAL_BIT2 m = n <= m)`,
+  `!n m. (ZERO <= n = T) /\
+         (BIT1 n <= ZERO = F) /\ 
+         (BIT2 n <= ZERO = F) /\
+         (BIT1 n <= BIT1 m = n <= m) /\
+         (BIT1 n <= BIT2 m = n <= m) /\
+         (BIT2 n <= BIT1 m = ~(m <= n)) /\
+         (BIT2 n <= BIT2 m = n <= m)`,
   SIMP_TAC bool_ss ([DOUBLE_FACTS, LESS_MONO_EQ, LESS_EQ_MONO] @
                     (map (REWRITE_RULE [NUMERAL_DEF])
                          [ZERO_LESS_EQ, NOT_SUC_LESS_EQ_0, NOT_LESS]) @
@@ -255,14 +253,12 @@ val _ = print "   (includes initiality theorem for bit functions)\n";
 
 val numeral_pre = store_thm(
   "numeral_pre",
-  --`(PRE ALT_ZERO = ALT_ZERO) /\
-     (PRE (NUMERAL_BIT1 ALT_ZERO) = ALT_ZERO) /\
-     (!n. PRE (NUMERAL_BIT1 (NUMERAL_BIT1 n)) =
-          NUMERAL_BIT2 (PRE (NUMERAL_BIT1 n))) /\
-     (!n. PRE (NUMERAL_BIT1 (NUMERAL_BIT2 n)) =
-          NUMERAL_BIT2 (NUMERAL_BIT1 n)) /\
-     (!n. PRE (NUMERAL_BIT2 n) = NUMERAL_BIT1 n)`--,
-  SIMP_TAC bool_ss [NUMERAL_BIT1, NUMERAL_BIT2, PRE, PRE_ADD,
+  --`(PRE ZERO = ZERO) /\
+     (PRE (BIT1 ZERO) = ZERO) /\
+     (!n. PRE (BIT1 (BIT1 n)) = BIT2 (PRE (BIT1 n))) /\
+     (!n. PRE (BIT1 (BIT2 n)) = BIT2 (BIT1 n)) /\
+     (!n. PRE (BIT2 n) = BIT1 n)`--,
+  SIMP_TAC bool_ss [BIT1, BIT2, PRE, PRE_ADD,
                     ADD_CLAUSES, ADD_ASSOC, PRE, ALT_ZERO]);
 
 (* we could just go on and prove similar rewrites for subtraction, but
@@ -276,11 +272,11 @@ val numeral_pre = store_thm(
 
 (* our measure function *)
 val our_M = Term
- `\f a. if a = ALT_ZERO then (zf:'a) else
-        if (?n. (a = NUMERAL_BIT1 n))
+ `\f a. if a = ZERO then (zf:'a) else
+        if (?n. (a = BIT1 n))
           then (b1f:num->'a->'a)
-                  (@n. a = NUMERAL_BIT1 n) (f (@n. a = NUMERAL_BIT1 n))
-          else b2f  (@n. a = NUMERAL_BIT2 n) (f (@n. a = NUMERAL_BIT2 n))`;
+                  (@n. a = BIT1 n) (f (@n. a = BIT1 n))
+          else b2f  (@n. a = BIT2 n) (f (@n. a = BIT2 n))`;
 
 
 fun AP_TAC (asl, g) =
@@ -304,9 +300,9 @@ val bit_initiality = store_thm(
   Term
   `!zf b1f b2f.
       ?f.
-        (f ALT_ZERO = zf) /\
-        (!n. f (NUMERAL_BIT1 n) = b1f n (f n)) /\
-        (!n. f (NUMERAL_BIT2 n) = b2f n (f n))`,
+        (f ZERO = zf) /\
+        (!n. f (BIT1 n) = b1f n (f n)) /\
+        (!n. f (BIT2 n) = b2f n (f n))`,
   REPEAT STRIP_TAC THEN
   ASSUME_TAC
     (MP (INST_TYPE [Type.beta |-> Type.alpha]
@@ -320,36 +316,35 @@ val bit_initiality = store_thm(
     GEN_TAC THEN
     FIRST_ASSUM (fn th => CONV_TAC (LHS_CONV (REWR_CONV th))) THEN
     SIMP_TAC bool_ss [numeral_eq] THEN AP_TAC THEN
-    SIMP_TAC bool_ss [relationTheory.RESTRICT_DEF, NUMERAL_BIT1] THEN
+    SIMP_TAC bool_ss [relationTheory.RESTRICT_DEF, BIT1] THEN
     ONCE_REWRITE_TAC [ADD_CLAUSES] THEN REWRITE_TAC [LESS_ADD_SUC],
     GEN_TAC THEN
     FIRST_ASSUM (fn th => CONV_TAC (LHS_CONV (REWR_CONV th))) THEN
     SIMP_TAC bool_ss [numeral_eq] THEN AP_TAC THEN
-    SIMP_TAC bool_ss [relationTheory.RESTRICT_DEF, NUMERAL_BIT2] THEN
+    SIMP_TAC bool_ss [relationTheory.RESTRICT_DEF, BIT2] THEN
     ONCE_REWRITE_TAC [ADD_CLAUSES] THEN REWRITE_TAC [LESS_ADD_SUC]
   ]);
 
 val bit_cases = prove(Term
-  `!n. (n = ALT_ZERO) \/ (?b1. n = NUMERAL_BIT1 b1) \/
-       (?b2. n = NUMERAL_BIT2 b2)`,
+  `!n. (n = ZERO) \/ (?b1. n = BIT1 b1) \/ (?b2. n = BIT2 b2)`,
 INDUCT_TAC THENL [
   SIMP_TAC bool_ss [ALT_ZERO],
   POP_ASSUM (STRIP_ASSUME_TAC) THEN POP_ASSUM SUBST_ALL_TAC THENL [
-    DISJ2_TAC THEN DISJ1_TAC THEN EXISTS_TAC (Term`ALT_ZERO`) THEN
+    DISJ2_TAC THEN DISJ1_TAC THEN EXISTS_TAC (Term`ZERO`) THEN
     REWRITE_TAC [numeral_suc],
     DISJ2_TAC THEN DISJ2_TAC THEN Q.EXISTS_TAC `b1` THEN
-    SIMP_TAC bool_ss [NUMERAL_BIT1, NUMERAL_BIT2, ADD_CLAUSES],
+    SIMP_TAC bool_ss [BIT1, BIT2, ADD_CLAUSES],
     DISJ2_TAC THEN DISJ1_TAC THEN Q.EXISTS_TAC `SUC b2` THEN
-    SIMP_TAC bool_ss [NUMERAL_BIT1, NUMERAL_BIT2, ADD_CLAUSES]
+    SIMP_TAC bool_ss [BIT1, BIT2, ADD_CLAUSES]
   ]
 ]);
 
 val old_style_bit_initiality = prove(Term
   `!zf b1f b2f.
       ?!f.
-        (f ALT_ZERO = zf) /\
-        (!n. f (NUMERAL_BIT1 n) = b1f (f n) n) /\
-        (!n. f (NUMERAL_BIT2 n) = b2f (f n) n)`,
+        (f ZERO = zf) /\
+        (!n. f (BIT1 n) = b1f (f n) n) /\
+        (!n. f (BIT2 n) = b2f (f n) n)`,
   REPEAT GEN_TAC THEN CONV_TAC EXISTS_UNIQUE_CONV THEN CONJ_TAC THENL [
     STRIP_ASSUME_TAC
       (Q.SPECL [`zf`, `\n a. b1f a n`, `\n a. b2f a n`] bit_initiality) THEN
@@ -361,10 +356,10 @@ val old_style_bit_initiality = prove(Term
     REPEAT_TCL STRIP_THM_THEN SUBST_ALL_TAC (SPEC_ALL bit_cases) THENL [
       ASM_SIMP_TAC bool_ss [],
       ASM_SIMP_TAC bool_ss [] THEN AP_TAC THEN AP_TAC THEN
-      FIRST_ASSUM MATCH_MP_TAC THEN SIMP_TAC bool_ss [NUMERAL_BIT1] THEN
+      FIRST_ASSUM MATCH_MP_TAC THEN SIMP_TAC bool_ss [BIT1] THEN
       ONCE_REWRITE_TAC [ADD_CLAUSES] THEN REWRITE_TAC [LESS_ADD_SUC],
       ASM_SIMP_TAC bool_ss [] THEN AP_TAC THEN AP_TAC THEN
-      FIRST_ASSUM MATCH_MP_TAC THEN SIMP_TAC bool_ss [NUMERAL_BIT2] THEN
+      FIRST_ASSUM MATCH_MP_TAC THEN SIMP_TAC bool_ss [BIT2] THEN
       ONCE_REWRITE_TAC [ADD_CLAUSES] THEN REWRITE_TAC [LESS_ADD_SUC]
     ]
   ]);
@@ -375,9 +370,9 @@ val old_style_bit_initiality = prove(Term
    function for the bit structure. *)
 
 val iBIT_cases = new_recursive_definition {
-  def = Term`(iBIT_cases ALT_ZERO zf bf1 bf2 = zf) /\
-             (iBIT_cases (NUMERAL_BIT1 n) zf bf1 bf2 = bf1 n) /\
-             (iBIT_cases (NUMERAL_BIT2 n) zf bf1 bf2 = bf2 n)`,
+  def = Term`(iBIT_cases ZERO zf bf1 bf2 = zf) /\
+             (iBIT_cases (BIT1 n) zf bf1 bf2 = bf1 n) /\
+             (iBIT_cases (BIT2 n) zf bf1 bf2 = bf2 n)`,
   name = "iBIT_cases",
   rec_axiom = bit_initiality};
 
@@ -399,32 +394,33 @@ val iDUB = new_definition("iDUB", Term`iDUB x = x + x`);
 
 val iSUB_DEF = new_recursive_definition {
   def = Term`
-    (iSUB b ALT_ZERO x = ALT_ZERO) /\
-    (iSUB b (NUMERAL_BIT1 n) x =
-       (b
-        => iBIT_cases x (NUMERAL_BIT1 n)
-           (* BIT1 m *) (\m. iDUB (iSUB T n m))
-           (* BIT2 m *) (\m. NUMERAL_BIT1 (iSUB F n m))
-        |  iBIT_cases x (iDUB n)
-           (* BIT1 m *) (\m. NUMERAL_BIT1 (iSUB F n m))
-           (* BIT2 m *) (\m. iDUB (iSUB F n m)))) /\
-    (iSUB b (NUMERAL_BIT2 n) x =
-       (b
-        => iBIT_cases x (NUMERAL_BIT2 n)
-           (* BIT1 m *) (\m. NUMERAL_BIT1 (iSUB T n m))
-           (* BIT2 m *) (\m. iDUB (iSUB T n m))
-        |  iBIT_cases x (NUMERAL_BIT1 n)
-           (* BIT1 m *) (\m. iDUB (iSUB T n m))
-           (* BIT2 m *) (\m. NUMERAL_BIT1 (iSUB F n m))))`,
+    (iSUB b ZERO x = ZERO) /\
+    (iSUB b (BIT1 n) x =
+       if b
+        then iBIT_cases x (BIT1 n)
+             (* BIT1 m *) (\m. iDUB (iSUB T n m))
+             (* BIT2 m *) (\m. BIT1 (iSUB F n m))
+        else iBIT_cases x (iDUB n)
+             (* BIT1 m *) (\m. BIT1 (iSUB F n m))
+             (* BIT2 m *) (\m. iDUB (iSUB F n m))) /\
+    (iSUB b (BIT2 n) x =
+       if b
+        then iBIT_cases x (BIT2 n)
+             (* BIT1 m *) (\m. BIT1 (iSUB T n m))
+             (* BIT2 m *) (\m. iDUB (iSUB T n m))
+        else iBIT_cases x (BIT1 n)
+             (* BIT1 m *) (\m. iDUB (iSUB T n m))
+             (* BIT2 m *) (\m. BIT1 (iSUB F n m)))`,
   name = "iSUB_DEF",
   rec_axiom = bit_initiality};
 
 val bit_induction = save_thm
-  ("bit_induction", Prim_rec.prove_induction_thm old_style_bit_initiality);
+  ("bit_induction", 
+   Prim_rec.prove_induction_thm old_style_bit_initiality);
 
 val iSUB_ZERO = prove(
-  Term`(!n b. iSUB b ALT_ZERO n = ALT_ZERO) /\ 
-         (!n. iSUB T n ALT_ZERO = n)`,
+  Term`(!n b. iSUB b ZERO n = ZERO) /\ 
+       (!n.   iSUB T n ZERO = n)`,
   SIMP_TAC bool_ss [iSUB_DEF] THEN GEN_TAC THEN
   STRUCT_CASES_TAC (Q.SPEC `n` bit_cases) THEN
   SIMP_TAC bool_ss [iSUB_DEF, iBIT_cases]);
@@ -439,27 +435,19 @@ val iSUB_ZERO = prove(
 val iSUB_THM = store_thm(
   "iSUB_THM",
   Term
-  `!b n m. (iSUB b ALT_ZERO x = ALT_ZERO) /\ 
-           (iSUB T n ALT_ZERO = n) /\
-           (iSUB F (NUMERAL_BIT1 n) ALT_ZERO = iDUB n) /\
-           (iSUB T (NUMERAL_BIT1 n) (NUMERAL_BIT1 m) =
-              iDUB (iSUB T n m)) /\
-           (iSUB F (NUMERAL_BIT1 n) (NUMERAL_BIT1 m) =
-              NUMERAL_BIT1 (iSUB F n m)) /\
-           (iSUB T (NUMERAL_BIT1 n) (NUMERAL_BIT2 m) =
-              NUMERAL_BIT1 (iSUB F n m)) /\
-           (iSUB F (NUMERAL_BIT1 n) (NUMERAL_BIT2 m) =
-              iDUB (iSUB F n m)) /\
+  `!b n m. (iSUB b ZERO x = ZERO) /\ 
+           (iSUB T n ZERO = n) /\
+           (iSUB F (BIT1 n) ZERO = iDUB n) /\
+           (iSUB T (BIT1 n) (BIT1 m) = iDUB (iSUB T n m)) /\
+           (iSUB F (BIT1 n) (BIT1 m) = BIT1 (iSUB F n m)) /\
+           (iSUB T (BIT1 n) (BIT2 m) = BIT1 (iSUB F n m)) /\
+           (iSUB F (BIT1 n) (BIT2 m) = iDUB (iSUB F n m)) /\
 
-           (iSUB F (NUMERAL_BIT2 n) ALT_ZERO = NUMERAL_BIT1 n) /\
-           (iSUB T (NUMERAL_BIT2 n) (NUMERAL_BIT1 m) =
-              NUMERAL_BIT1 (iSUB T n m)) /\
-           (iSUB F (NUMERAL_BIT2 n) (NUMERAL_BIT1 m) =
-              iDUB (iSUB T n m)) /\
-           (iSUB T (NUMERAL_BIT2 n) (NUMERAL_BIT2 m) =
-              iDUB (iSUB T n m)) /\
-           (iSUB F (NUMERAL_BIT2 n) (NUMERAL_BIT2 m) =
-              NUMERAL_BIT1 (iSUB F n m))`,
+           (iSUB F (BIT2 n) ZERO = BIT1 n) /\
+           (iSUB T (BIT2 n) (BIT1 m) = BIT1 (iSUB T n m)) /\
+           (iSUB F (BIT2 n) (BIT1 m) = iDUB (iSUB T n m)) /\
+           (iSUB T (BIT2 n) (BIT2 m) = iDUB (iSUB T n m)) /\
+           (iSUB F (BIT2 n) (BIT2 m) = BIT1 (iSUB F n m))`,
   SIMP_TAC bool_ss [iSUB_DEF, iBIT_cases, iSUB_ZERO]);
 
 (* rewrites for relational expressions that can be used under
@@ -512,16 +500,16 @@ val iSUB_correct = prove(
     SIMP_TAC bool_ss [SUB, iSUB_ZERO, ALT_ZERO],
     SIMP_TAC bool_ss [iSUB_DEF] THEN GEN_TAC THEN
     STRUCT_CASES_TAC (Q.SPEC `m` bit_cases) THENL [
-      SIMP_TAC bool_ss [SUB_0, iBIT_cases, iDUB, NUMERAL_BIT1, ALT_ZERO] THEN
+      SIMP_TAC bool_ss [SUB_0, iBIT_cases, iDUB, BIT1, ALT_ZERO] THEN
       SIMP_TAC bool_ss [ADD_ASSOC, SUB_elim],
       SIMP_TAC bool_ss [iBIT_cases, numeral_lt, numeral_lte] THEN
-      ASM_SIMP_TAC bool_ss [NUMERAL_BIT2, NUMERAL_BIT1, PRE_SUB,
+      ASM_SIMP_TAC bool_ss [BIT2, BIT1, PRE_SUB,
         SUB_LEFT_SUC, SUB_MONO_EQ, SUB_LEFT_ADD, SUB_RIGHT_ADD, SUB_RIGHT_SUB,
         ADD_CLAUSES, less_less_eqs, LESS_MONO_EQ, GSYM LESS_OR_EQ, iDUB,
         DOUBLE_FACTS] THEN CONJ_TAC THEN
       SIMP_TAC bool_ss [COND_OUT_THMS, ADD_CLAUSES, sub_facts],
-      ASM_SIMP_TAC bool_ss [iBIT_cases, numeral_lt, NUMERAL_BIT1,
-        NUMERAL_BIT2, PRE_SUB, SUB_LEFT_SUC, SUB_MONO_EQ, SUB_LEFT_ADD,
+      ASM_SIMP_TAC bool_ss [iBIT_cases, numeral_lt, BIT1,
+        BIT2, PRE_SUB, SUB_LEFT_SUC, SUB_MONO_EQ, SUB_LEFT_ADD,
         SUB_RIGHT_ADD, SUB_RIGHT_SUB, ADD_CLAUSES, less_less_eqs, iDUB,
         DOUBLE_FACTS, LESS_EQ_MONO] THEN
       CONJ_TAC THEN
@@ -530,14 +518,14 @@ val iSUB_correct = prove(
     GEN_TAC THEN STRUCT_CASES_TAC (Q.SPEC `m` bit_cases) THEN
     ASM_SIMP_TAC bool_ss [iBIT_cases, numeral_lte, numeral_lt, ALT_ZERO,
                           iSUB_DEF, SUB_0] THENL [
-      SIMP_TAC bool_ss [sub_facts, NUMERAL_BIT2, NUMERAL_BIT1, ADD_CLAUSES,
+      SIMP_TAC bool_ss [sub_facts, BIT2, BIT1, ADD_CLAUSES,
                         SUB_MONO_EQ, SUB_0],
-      ASM_SIMP_TAC bool_ss [NOT_LESS, NUMERAL_BIT1, NUMERAL_BIT2, iDUB,
+      ASM_SIMP_TAC bool_ss [NOT_LESS, BIT1, BIT2, iDUB,
         ADD_CLAUSES, SUB_MONO_EQ, INV_SUC_EQ, SUB_LEFT_SUC, SUB_RIGHT_SUB,
         SUB_LEFT_SUB, SUB_LEFT_ADD, SUB_RIGHT_ADD, less_less_eqs] THEN
       CONJ_TAC THEN
       SIMP_TAC bool_ss [COND_OUT_THMS, ADD_CLAUSES, sub_facts, NUMERAL_DEF],
-      ASM_SIMP_TAC bool_ss [NOT_LESS, NUMERAL_BIT1, NUMERAL_BIT2, iDUB,
+      ASM_SIMP_TAC bool_ss [NOT_LESS, BIT1, BIT2, iDUB,
         ADD_CLAUSES, SUB_MONO_EQ, INV_SUC_EQ, SUB_LEFT_SUC, SUB_RIGHT_SUB,
         SUB_LEFT_SUB, SUB_LEFT_ADD, SUB_RIGHT_ADD, less_less_eqs] THEN
       CONJ_TAC THEN
@@ -557,10 +545,10 @@ val NOT_ZERO = arithmeticTheory.NOT_ZERO_LT_ZERO;
 
 val iDUB_removal = store_thm(
   "iDUB_removal",
-  Term`!n. (iDUB (NUMERAL_BIT1 n) = NUMERAL_BIT2 (iDUB n)) /\
-           (iDUB (NUMERAL_BIT2 n) = NUMERAL_BIT2 (NUMERAL_BIT1 n)) /\
-           (iDUB ALT_ZERO = ALT_ZERO)`,
-  SIMP_TAC bool_ss [iDUB, NUMERAL_BIT2, NUMERAL_BIT1, PRE_SUB1,
+  Term`!n. (iDUB (BIT1 n) = BIT2 (iDUB n)) /\
+           (iDUB (BIT2 n) = BIT2 (BIT1 n)) /\
+           (iDUB ZERO = ZERO)`,
+  SIMP_TAC bool_ss [iDUB, BIT2, BIT1, PRE_SUB1,
                     ADD_CLAUSES, ALT_ZERO]);
 
 (* rewriting for multiplication *)
@@ -570,11 +558,11 @@ val _ = print "Developing numeral rewrites for multiplication\n"
 val numeral_mult = store_thm(
   "numeral_mult", Term
   `!n m.
-     (ALT_ZERO * n = ALT_ZERO) /\ 
-     (n * ALT_ZERO = ALT_ZERO) /\
-     (NUMERAL_BIT1 n * m = iZ (iDUB (n * m) + m)) /\
-     (NUMERAL_BIT2 n * m = iDUB (iZ (n * m + m)))`,
-  SIMP_TAC bool_ss [NUMERAL_BIT1, NUMERAL_BIT2, iDUB, RIGHT_ADD_DISTRIB, iZ,
+     (ZERO * n = ZERO) /\ 
+     (n * ZERO = ZERO) /\
+     (BIT1 n * m = iZ (iDUB (n * m) + m)) /\
+     (BIT2 n * m = iDUB (iZ (n * m + m)))`,
+  SIMP_TAC bool_ss [BIT1, BIT2, iDUB, RIGHT_ADD_DISTRIB, iZ,
                     MULT_CLAUSES, ADD_CLAUSES, ALT_ZERO] THEN
   REPEAT GEN_TAC THEN CONV_TAC (AC_CONV (ADD_ASSOC, ADD_SYM)));
 
@@ -591,10 +579,10 @@ val iSQR = new_definition("iSQR", Term`iSQR x = x * x`);
 
 val numeral_exp = store_thm(
   "numeral_exp", Term
-  `(!n. n EXP ALT_ZERO = NUMERAL_BIT1 ALT_ZERO) /\
-   (!n m. n EXP (NUMERAL_BIT1 m) = n * iSQR (n EXP m)) /\
-   (!n m. n EXP (NUMERAL_BIT2 m) = iSQR n * iSQR (n EXP m))`,
-  SIMP_TAC bool_ss [NUMERAL_BIT1, iSQR, NUMERAL_BIT2, EXP_ADD, EXP,
+  `(!n. n EXP ZERO = BIT1 ZERO) /\
+   (!n m. n EXP (BIT1 m) = n * iSQR (n EXP m)) /\
+   (!n m. n EXP (BIT2 m) = iSQR n * iSQR (n EXP m))`,
+  SIMP_TAC bool_ss [BIT1, iSQR, BIT2, EXP_ADD, EXP,
                     ADD_CLAUSES, ALT_ZERO, NUMERAL_DEF] THEN
   REPEAT STRIP_TAC THEN CONV_TAC (AC_CONV(MULT_ASSOC, MULT_SYM)));
 
@@ -602,42 +590,36 @@ val _ = print "Even-ness and odd-ness of numerals\n"
 
 val numeral_evenodd = store_thm(
   "numeral_evenodd",
-  Term`!n. EVEN ALT_ZERO /\ EVEN (NUMERAL_BIT2 n) /\ ~EVEN (NUMERAL_BIT1 n) /\
-           ~ODD ALT_ZERO /\ ~ODD (NUMERAL_BIT2 n) /\ ODD (NUMERAL_BIT1 n)`,
-  SIMP_TAC bool_ss [NUMERAL_BIT1, ALT_ZERO, NUMERAL_BIT2, ADD_CLAUSES,
+  Term`!n. EVEN ZERO /\ EVEN (BIT2 n) /\ ~EVEN (BIT1 n) /\
+           ~ODD ZERO /\ ~ODD (BIT2 n) /\ ODD (BIT1 n)`,
+  SIMP_TAC bool_ss [BIT1, ALT_ZERO, BIT2, ADD_CLAUSES,
                     EVEN, ODD, EVEN_ADD, ODD_ADD]);
 
 
-val numeral_fact = store_thm(
-  "numeral_fact",
+val numeral_fact = store_thm
+("numeral_fact",
   Term `(FACT 0 = 1) /\
-        (!n. FACT (NUMERAL (NUMERAL_BIT1 n)) =
-                  (NUMERAL (NUMERAL_BIT1 n)) *
-                  FACT (PRE (NUMERAL (NUMERAL_BIT1 n)))) /\
-        (!n. FACT (NUMERAL (NUMERAL_BIT2 n)) =
-                  (NUMERAL (NUMERAL_BIT2 n)) *
-                  FACT (NUMERAL (NUMERAL_BIT1 n)))`,
+        (!n. FACT (NUMERAL (BIT1 n)) = NUMERAL (BIT1 n) * FACT (PRE(NUMERAL(BIT1 n)))) /\
+        (!n. FACT (NUMERAL (BIT2 n)) = NUMERAL (BIT2 n) * FACT (NUMERAL (BIT1 n)))`,
  REPEAT STRIP_TAC THEN REWRITE_TAC [FACT] THEN
  (STRIP_ASSUME_TAC (SPEC (Term`n:num`) num_CASES) THENL [
     ALL_TAC,
     POP_ASSUM SUBST_ALL_TAC
   ] THEN ASM_REWRITE_TAC[FACT,PRE,NOT_SUC, NUMERAL_DEF,
-                         NUMERAL_BIT1, NUMERAL_BIT2, ADD_CLAUSES]));
+                         BIT1, BIT2, ADD_CLAUSES]));
 
 
 val numeral_funpow = store_thm(
   "numeral_funpow",
   Term `(FUNPOW f 0 x = x) /\
-        (FUNPOW f (NUMERAL (NUMERAL_BIT1 n)) x =
-          FUNPOW f (PRE (NUMERAL (NUMERAL_BIT1 n))) (f x)) /\
-        (FUNPOW f (NUMERAL (NUMERAL_BIT2 n)) x =
-          FUNPOW f (NUMERAL (NUMERAL_BIT1 n)) (f x))`,
+        (FUNPOW f (NUMERAL (BIT1 n)) x = FUNPOW f (PRE (NUMERAL (BIT1 n))) (f x)) /\
+        (FUNPOW f (NUMERAL (BIT2 n)) x = FUNPOW f (NUMERAL (BIT1 n)) (f x))`,
  REPEAT STRIP_TAC THEN REWRITE_TAC [FUNPOW] THEN
  (STRIP_ASSUME_TAC (SPEC (Term`n:num`) num_CASES) THENL [
     ALL_TAC,
     POP_ASSUM SUBST_ALL_TAC
   ] THEN  ASM_REWRITE_TAC[FUNPOW,PRE,ADD_CLAUSES, NUMERAL_DEF,
-                          NUMERAL_BIT1, NUMERAL_BIT2]));
+                          BIT1, BIT2]));
 
 val numeral_MIN = store_thm(
   "numeral_MIN",
@@ -675,15 +657,15 @@ val (even,odd) =
      (LIST_CONJ [a',b',c'], LIST_CONJ [d',e',f'])
   end;
 
-val _ = ConstMapML.prim_insert(Term`0n`,("num","ALT_ZERO",Type`:num`));
+val _ = ConstMapML.prim_insert(Term`0n`,("num","ZERO",Type`:num`));
 
 val _ = 
   let open Drop arithmeticTheory whileTheory
   in 
     exportML("num",
-     DATATYPE (ParseDatatype.parse `num = ALT_ZERO 
-                                        | NUMERAL_BIT1 of num 
-                                        | NUMERAL_BIT2 of num`)
+     DATATYPE (ParseDatatype.parse `num = ZERO 
+                                        | BIT1 of num 
+                                        | BIT2 of num`)
       ::
      DEFN NUMERAL_DEF ::
       map (DEFN o PURE_REWRITE_RULE [NUMERAL_DEF])
@@ -702,7 +684,7 @@ val _ = adjoin_to_theory
       fun NL() = PP.add_newline ppstrm
   in S "val _ = ConstMapML.prim_insert "; NL();
      S "         (Term.prim_mk_const{Name=\"0\",Thy=\"num\"},"; NL();
-     S "          (\"num\",\"ALT_ZERO\",Type.mk_type(\"num\",[])));";
+     S "          (\"num\",\"ZERO\",Type.mk_type(\"num\",[])));";
      NL(); NL()
   end)};
          
