src/real/realScript.sml
@@ -3372,14 +3372,14 @@ val mult_ints = store_thm(
 val pow_rat = store_thm(
   "pow_rat",
   ``(x pow 0 = 1) /\
-    (0 pow (NUMERAL (NUMERAL_BIT1 n)) = 0) /\
-    (0 pow (NUMERAL (NUMERAL_BIT2 n)) = 0) /\
+    (0 pow (NUMERAL (BIT1 n)) = 0) /\
+    (0 pow (NUMERAL (BIT2 n)) = 0) /\
     (&(NUMERAL a) pow (NUMERAL n) = &(NUMERAL a EXP NUMERAL n)) /\
     (~&(NUMERAL a) pow (NUMERAL n) =
       (if ODD (NUMERAL n) then (~) else (\x.x))
       (&(NUMERAL a EXP NUMERAL n))) /\
     ((x / y) pow n = (x pow n) / (y pow n))``,
-  SIMP_TAC bool_ss [pow, NUMERAL_DEF, NUMERAL_BIT1, NUMERAL_BIT2, POW_ADD,
+  SIMP_TAC bool_ss [pow, NUMERAL_DEF, BIT1, BIT2, POW_ADD,
                     ALT_ZERO, ADD_CLAUSES, REAL_MUL, MULT_CLAUSES,
                     REAL_MUL_RZERO, REAL_OF_NUM_POW, REAL_POW_DIV, EXP] THEN
   Induct_on `n` THEN ASM_SIMP_TAC bool_ss [pow, ODD, EXP] THEN
